internal del not working

list.dfy
@@ -3,78 +3,150 @@ include "Node.dfy"
 
 
 // analogue to __list_add
-method internal_list_add(new_node: Node, prev: Node, next: Node)
-  requires Valid(new_node) && Valid(prev) && Valid(next) // must be valid nodes
-  requires Singleton(new_node) // must be a new node
-  requires new_node != prev && new_node != next // all are different nodes
-  requires prev.nodes == next.nodes // same linked list
-  requires prev.next == next // next should be immediately after
-  modifies next, prev, new_node, multiset(prev.nodes)
-  ensures Valid(new_node)
-  ensures Valid(prev)
-  ensures Valid(next)
-  ensures prev.nodes == next.nodes == new_node.nodes
-  ensures |prev.nodes| == |old(prev.nodes)|+1
+// method internal_list_add(new_node: Node, prev: Node, next: Node)
+//   requires Valid(new_node) && Valid(prev) && Valid(next) // must be valid nodes
+//   requires Singleton(new_node) // must be a new node
+//   requires new_node != prev && new_node != next // all are different nodes
+//   requires prev.nodes == next.nodes // same linked list
+//   requires prev.next == next // next should be immediately after
+//   modifies next, prev, new_node, multiset(prev.nodes)
+//   ensures Valid(new_node)
+//   ensures Valid(prev)
+//   ensures Valid(next)
+//   ensures prev.nodes == next.nodes == new_node.nodes
+//   ensures |prev.nodes| == |old(prev.nodes)|+1
+// {
+//   next.prev := new_node;
+//   new_node.next := next;
+//   new_node.prev := prev;
+//   prev.next := new_node;
+
+//   // Proof of the above
+//   // Consider 2 cases - when prev is the very last node, and when it isn't, to handle appending the node correctly
+//   // NOTE: the nodes object is shared so directly modifying it will affect everyone. Be careful!
+
+//   assert prev.nodes[IndexOf(prev.nodes, prev)] == prev;
+//   assert next.nodes[IndexOf(next.nodes, next)] == next;
+//   var prev_idx := IndexOf(prev.nodes, prev);
+
+//   if prev_idx == |prev.nodes|-1 {
+//     assert prev.nodes[0] == next;
+//     ghost var new_nodes := prev.nodes + [new_node];
+//     forall a' | a' in new_nodes {
+//       a'.nodes := new_nodes;
+//     }
+//   } else {
+//     assert prev.nodes[prev_idx+1] == next;
+//     ghost var new_nodes := prev.nodes[..(prev_idx+1)] + [new_node] + prev.nodes[(prev_idx+1)..];
+//     prev.nodes := new_nodes; // not sure why this is needed
+//     forall a' | a' in new_nodes {
+//       a'.nodes := new_nodes;
+//     }
+//   }
+// }
+
+// method list_add(new_node: Node, head: Node)
+//   requires Valid(new_node)
+//   requires Valid(head)
+//   requires Singleton(new_node)
+//   requires new_node !in head.nodes
+//   modifies new_node, head, multiset(head.nodes)
+// {
+//   var next := head.get_next();
+//   internal_list_add(new_node, head, next);
+// }
+
+// method list_add_tail(new_node: Node, head: Node)
+//   requires Valid(new_node)
+//   requires Valid(head)
+//   requires Singleton(new_node)
+//   requires new_node !in head.nodes
+//   modifies new_node, head, multiset(head.nodes)
+// {
+//   assert head.nodes[(IndexOf(head.nodes, head)+|head.nodes|-1) % |head.nodes|] == head.prev;
+//   internal_list_add(new_node, head.prev, head);
+// }
+
+ghost predicate same_linked_list(nodes: seq<Node>)
+requires |nodes| >= 1 
+reads multiset(nodes)
 {
-  next.prev := new_node;
-  new_node.next := next;
-  new_node.prev := prev;
-  prev.next := new_node;
-
-  // Proof of the above
-  // Consider 2 cases - when prev is the very last node, and when it isn't, to handle appending the node correctly
-  // NOTE: the nodes object is shared so directly modifying it will affect everyone. Be careful!
-
-  assert prev.nodes[IndexOf(prev.nodes, prev)] == prev;
-  assert next.nodes[IndexOf(next.nodes, next)] == next;
-  var prev_idx := IndexOf(prev.nodes, prev);
-
-  if prev_idx == |prev.nodes|-1 {
-    assert prev.nodes[0] == next;
-    ghost var new_nodes := prev.nodes + [new_node];
-    forall a' | a' in new_nodes {
-      a'.nodes := new_nodes;
-    }
-  } else {
-    assert prev.nodes[prev_idx+1] == next;
-    ghost var new_nodes := prev.nodes[..(prev_idx+1)] + [new_node] + prev.nodes[(prev_idx+1)..];
-    prev.nodes := new_nodes; // not sure why this is needed
-    forall a' | a' in new_nodes {
-      a'.nodes := new_nodes;
-    }
-  }
+  var ghost_nodes := nodes[0].nodes;
+  forall node' :: node' in nodes ==> node'.nodes == ghost_nodes
 }
 
-method list_add(new_node: Node, head: Node)
-  requires Valid(new_node)
-  requires Valid(head)
-  requires Singleton(new_node)
-  requires new_node !in head.nodes
-  modifies new_node, head, multiset(head.nodes)
-{
-  assert head.nodes[(IndexOf(head.nodes, head)+1) % |head.nodes|] == head.next;
-  internal_list_add(new_node, head, head.next);
-}
+// method internal_list_del(prev: Node, next: Node)
+//   requires prev.Valid() && next.Valid()
+//   requires prev.next.next == next
+//   requires prev != prev.next && prev.next != next
+//   requires same_linked_list([prev, next])
+//   modifies prev, next, prev.next, multiset(prev.nodes)
+//   ensures prev.Valid()
+//   ensures next.Valid()
+//   ensures same_linked_list([prev, next])
+//   ensures (
+//     var idx := IndexOf(old(prev.nodes), prev);
+//     && (idx == |prev.nodes|-1 ==> prev.nodes == old(prev.nodes[1..])) // prev is last, removed val is first index
+//     && (idx == |prev.nodes|-2 ==> prev.nodes == old(prev.nodes[..|prev.nodes|-1])) // prev is second last, removed is the last element
+//     && (0 <= idx < |old(prev.nodes)|-2 ==> prev.nodes == old(prev.nodes[..idx+1])+old(prev.nodes[idx+2..])) // anything else, then join arr till prev_idx] + [prev_idx+2..]
+//   )
+// {
+//   ghost var prev_idx := IndexOf(prev.nodes, prev);
+//   ghost var next_idx := IndexOf(prev.nodes, next);
+//   ghost var len := |prev.nodes|;
 
-method list_add_tail(new_node: Node, head: Node)
-  requires Valid(new_node)
-  requires Valid(head)
-  requires Singleton(new_node)
-  requires new_node !in head.nodes
-  modifies new_node, head, multiset(head.nodes)
-{
-  assert head.nodes[(IndexOf(head.nodes, head)+|head.nodes|-1) % |head.nodes|] == head.prev;
-  internal_list_add(new_node, head.prev, head);
-}
+//   var prev_next := prev.next; // maintain reference to removed node
+//   next.prev := prev;
+//   prev.next := next;
+
+//   // 3 cases - prev is the last node, the second last node, or any other node
+//   // in each assert the position of prev_next and next, then proceed to remove prev_next from the list
+
+//   if prev_idx == len - 1 {
+//     assert prev.nodes[0] == prev_next;
+//     assert prev.nodes[1] == next;
+
+//     var new_nodes := prev.nodes[1..];
+//     prev.nodes := new_nodes;
+//     forall a' | a' in new_nodes {
+//       a'.nodes := new_nodes;
+//     }
+//     assert prev.nodes[0] == next;
+//   } else if prev_idx == len - 2 {
+//     assert prev_idx != |prev.nodes|-1; 
+//     assert prev_idx != |prev.nodes|-1;
+//     assert prev.nodes[0] == next;
+//     assert prev.nodes[|prev.nodes|-1] == prev_next;
+
+//     var new_nodes := prev.nodes[..prev_idx+1];
+//     forall a' | a' in new_nodes {
+//       a'.nodes := new_nodes;
+//     }
+//   } else {
+//     assert 0 <= prev_idx < |prev.nodes|-2; 
+//     assert prev.nodes[prev_idx+1] == prev_next;
+//     assert prev.nodes[prev_idx+2] == next;
+//     assert next_idx == prev_idx+2;
+
+//     var splice_till_prev := prev.nodes[..prev_idx+1];
+//     var splice_from_next := prev.nodes[next_idx..];
+//     var new_nodes := splice_till_prev + splice_from_next;
+//     assert |new_nodes| >= 2;
+//     prev.nodes := new_nodes;
+//     forall a' | a' in new_nodes {
+//       a'.nodes := new_nodes;
+//     }
+//   }
+// }
 
 method internal_list_del(prev: Node, next: Node)
-  requires Valid(prev) && Valid(next) && Valid(prev.next)
+  requires prev.Valid() && next.Valid() && prev.next.Valid()
   requires prev.next.next == next
   requires prev != prev.next && prev.next != next
   requires prev.nodes == next.nodes == prev.next.nodes
   modifies prev, next, prev.next, multiset(prev.nodes)
-  ensures Valid(prev)
-  ensures Valid(next)
+  ensures prev.Valid()
+  ensures next.Valid()
   ensures prev.next == next
   ensures next.prev == prev
   ensures prev.nodes == next.nodes
@@ -134,20 +206,20 @@ method internal_list_del(prev: Node, next: Node)
 // ensures Valid(entry.prev)
 // ensures Valid(entry.next)
 // {
-//   var entry_next := entry.next;
-//   var entry_prev := entry.prev;
+//   var entry_next := entry.get_next();
+//   var entry_prev := entry.get_prev();
 
 //   // assert entry != entry.prev && entry != entry.next  ==> |entry.nodes| >= 2;
-//   assert entry.nodes[get_prev_seq_idx(entry.nodes, IndexOf(entry.nodes, entry))] == entry.prev;
-//   assert entry.nodes[get_next_seq_idx(entry.nodes, IndexOf(entry.nodes, entry))] == entry.next;
+//   // assert entry.nodes[get_prev_seq_idx(entry.nodes, IndexOf(entry.nodes, entry))] == entry_prev;
+//   // assert entry.nodes[get_next_seq_idx(entry.nodes, IndexOf(entry.nodes, entry))] == entry_next;
   
-//   assert Valid(entry) && entry != entry.prev ==> |entry.nodes| >= 2;
+//   // assert Valid(entry) && entry != entry.prev ==> |entry.nodes| >= 2;
 //   // assert Valid(entry.prev) && Valid(entry) && entry.nodes == entry.prev.nodes ==> entry.prev.next == entry;
 //   // assert Valid(entry.next) && Valid(entry) && entry.nodes == entry.next.nodes ==> entry.next.prev == entry;
 //   // assert entry.prev.next.next == entry.next;
 //   // assert entry.next.prev.prev == entry.prev;
 
-//   internal_list_del(entry.prev, entry.next); 
+//   internal_list_del(entry_prev, entry_next); 
 
-//   assert |entry.prev.nodes| == |entry.nodes| - 1;
+//   // assert |entry.prev.nodes| == |entry.nodes| - 1;
 // }
