node.dfy
@@ -6,7 +6,7 @@ class Node {
   ghost var nodes: seq<Node>
   // int nat seq<Node> map<node> set<Node>
   constructor()
-    ensures Valid(this)
+    ensures Valid()
     ensures this == this.nodes[0]
     ensures Singleton(this)
   {
@@ -14,32 +14,65 @@ class Node {
     next := this;
     nodes := [ this ];
   }
+
+  // Validity of a link in a cicular linked list
+  ghost predicate Valid()
+    reads this, multiset(nodes)
+  {
+    var nodes := this.nodes;
+
+    && |nodes| > 0
+    && (this in multiset(nodes)) // self is present in the set of nodes
+    && (forall node' :: node' in nodes ==> node'.nodes == nodes) // all nodes are same in the chain
+    && NoDupes(nodes) // no duplicates in the chain (they are pointers)
+    && (forall i :: 0 <= i < |nodes| - 1 ==> nodes[i].next == nodes[i+1]) // assert that every next pointer is in the next index
+    && nodes[|nodes|-1].next == nodes[0] // except the very last one that wraps to the first one
+    && (forall i :: 1 <= i < |nodes| ==> nodes[i].prev == nodes[i-1]) // assert that every prev pointer is in the prev index
+    && nodes[0].prev == nodes[|nodes|-1] // except the very first one that wraps to the last one
+  }
+
+  method get_prev() returns (prev: Node)
+    requires Valid()
+    ensures prev == this.prev
+    ensures prev.Valid()
+  {
+    prev_is_valid();
+    return this.prev;
+  }
+
+  method get_next() returns (next: Node)
+    requires Valid()
+    ensures next == this.next
+    ensures next.Valid()
+    ensures next.nodes == nodes
+  {
+    next_is_valid();
+    return this.next;
+  }
+
+  lemma next_is_valid()
+    requires Valid()
+    ensures next.Valid()
+    ensures next.nodes == nodes
+  {
+    assert this.nodes[get_next_seq_idx(this.nodes, IndexOf(this.nodes, this))] == this.next;
+  }
+
+  lemma prev_is_valid()
+    requires Valid()
+    ensures prev.Valid()
+    ensures prev.nodes == nodes {
+    assert this.nodes[get_prev_seq_idx(this.nodes, IndexOf(this.nodes, this))] == this.prev;
+  }
 }
 
 // implies that this node is not connected to any other nodes.
 predicate Singleton(n: Node)
-  requires Valid(n)
+  requires n.Valid()
   ensures Singleton(n) ==> n.nodes == [ n ]
   reads n, n.nodes
 {
   ghost var i := IndexOf(n.nodes, n);
   assert n.next == n.nodes[(i + 1) % |n.nodes|];
   n.prev == n.next == n
-}
-
-// Validity of a link in a cicular linked list
-ghost predicate Valid(node: Node)
-  reads node
-  reads node.nodes
-{
-  var nodes := node.nodes;
-
-  && |nodes| > 0
-  && (node in multiset(nodes)) // self is present in the set of nodes
-  && (forall node' :: node' in nodes ==> node'.nodes == nodes) // all nodes are same in the chain
-  && NoDupes(nodes) // no duplicates in the chain (they are pointers)
-  && (forall i :: 0 <= i < |nodes| - 1 ==> nodes[i].next == nodes[i+1]) // assert that every next pointer is in the next index
-  && nodes[|nodes|-1].next == nodes[0] // except the very last one that wraps to the first one
-  && (forall i :: 1 <= i < |nodes| ==> nodes[i].prev == nodes[i-1]) // assert that every prev pointer is in the prev index
-  && nodes[0].prev == nodes[|nodes|-1] // except the very first one that wraps to the last one
 }
